fairis/heap_lang/examples/even_odd/action_model.v
@@ -1,0 +1,336 @@
+From trillium.fairness Require Import fairness.
+
+  Lemma ex2_comm {A B: Type} (P: A -> B -> Prop):
+    (exists (a: A) (b: B), P a b) <-> (exists (b: B) (a: A), P a b).
+  Proof. 
+    split; intros (?&?&?); eauto. 
+  Qed. 
+
+  Lemma iff_and_impl_helper {A B: Prop} (AB: A -> B):
+    A /\ B <-> A.
+  Proof. tauto. Qed.     
+
+  Lemma ex_det_iff {A: Type} (P: A -> Prop) a
+    (DET: forall a', P a' -> a' = a):
+    (exists a', P a') <-> P a.
+  Proof. 
+    split; [| by eauto].
+    intros [? ?]. erewrite <- DET; eauto.
+  Qed. 
+
+Section ActionModel.
+
+  (* Class PreModel := { *)
+  (*     pmState: Type; *)
+  (*     pmPubA: Type; *)
+  (*     pmPrivA: Type; *)
+  (*     pmA: Type := pmPubA + pmPrivA; *)
+  (*     pmTrans: pmState -> option pmA -> pmState -> Prop; *)
+  (* }. *)
+    
+  (* Class PreModel (pmPubA: Type) := { *)
+  (*     pmState: Type; *)
+  (*     pmPrivA: Type; *)
+  (*     pmRole: Type; *)
+  (*     pmA: Type := option pmPubA + pmPrivA; *)
+  (*     pmTrans: pmState -> pmA * pmRole -> pmState -> Prop; *)
+  (* }. *)
+
+  Record ActionModel := {
+      amSt: Type;
+      (* amPubA: Type; *)
+      (* amPrivA: Type; *)
+      (* amA: Type := amPubA + amPrivA; *)
+      amA: Type;
+      amRole: Type;
+      amTrans: amSt -> amA * option amRole -> amSt -> Prop;
+  }.
+
+  Arguments amTrans {_}. 
+
+  Definition AM_strong_lr (AM: ActionModel) `{Countable (amRole AM)} :=
+    {lr: amSt AM -> gset (option (amRole AM)) |
+      forall st oρ, oρ ∈ lr st <-> exists a st', amTrans st (a, oρ) st'}.
+
+  Definition AM_fin_branch' (AM: ActionModel) := 
+    {next_steps': amSt AM -> list (amSt AM * amA AM * option (amRole AM)) 
+     | forall s1 s2 a oρ, amTrans s1 (a, oρ) s2 -> (s2, a, oρ) ∈ next_steps' s1}.
+
+  Definition AM_step_dec (AM: ActionModel) :=
+    forall s1 a oρ s2, Decision (@amTrans AM s1 (a, oρ) s2).
+
+  Definition AM_fin_branch (AM: ActionModel) := 
+    {next_steps: amSt AM -> list (amSt AM * amA AM * option (amRole AM)) 
+     | forall s1 s2 a oρ, amTrans s1 (a, oρ) s2 <-> (s2, a, oρ) ∈ next_steps s1}.
+
+  Lemma AM_fin_branch_dec (AM: ActionModel)
+    (FIN: AM_fin_branch' AM) (DEC: AM_step_dec AM):
+    AM_fin_branch AM.
+  Proof. 
+    destruct FIN as [ns' FIN]. 
+    exists (fun s => filter (fun '(s2, a, oρ) => @bool_decide _ (DEC s a oρ s2)) (ns' s)).
+    intros. rewrite elem_of_list_filter. rewrite bool_decide_spec.
+    symmetry. apply iff_and_impl_helper. intuition.
+  Qed.
+
+  (* TODO: move *)
+  Lemma ex_prod {A B: Type} (P: A * B -> Prop):
+    (exists ab, P ab) <-> (exists a b, P (a, b)).
+  Proof.
+    split.
+    - intros [[??] ?]. eauto.
+    - intros (?&?&?). eauto.
+  Qed. 
+
+  Lemma fin_branch_strong (AM: ActionModel) `{Countable (amRole AM)}
+    (FIN: AM_fin_branch' AM) (DEC: AM_step_dec AM):
+    AM_strong_lr AM.
+  Proof.
+    eapply AM_fin_branch_dec in FIN as [ns FIN]; auto.
+    exists (fun s => list_to_set ((fun '(_, _, oρ) => oρ) <$> ns s)). 
+    intros. rewrite elem_of_list_to_set. rewrite elem_of_list_fmap.
+    do 2 rewrite ex_prod.
+    setoid_rewrite ex_det_iff with (a := oρ); [| by intuition].
+    rewrite ex2_comm. do 2 (apply exist_proper; intros).
+    rewrite FIN. tauto.
+  Qed. 
+
+  (* TODO: move *)
+  (* useful for defining live_roles of AM *)
+  Definition extract_Somes {A: Type} (l: list (option A)): list A :=
+    flat_map (from_option (fun a => [a]) []) l.
+
+  Lemma extract_Somes_spec {A: Type} (l: list (option A)):
+    forall a, In (Some a) l <-> In a (extract_Somes l).
+  Proof. 
+    intros. rewrite /extract_Somes.
+    rewrite in_flat_map_Exists.
+    rewrite List.Exists_exists. simpl.
+    erewrite ex_det_iff with (a := Some a). 
+    2: { intros ? [? ?]. destruct a'; try done.
+         simpl in H0. set_solver. }
+    simpl. set_solver.
+  Qed.
+
+  Definition extract_Somes_gset `{Countable A} (s: gset (option A)): gset A :=
+    list_to_set ∘ extract_Somes ∘ elements $ s. 
+  
+  Lemma extract_Somes_gset_spec `{Countable A} (s: gset (option A)):
+    forall a, Some a ∈ s <-> a ∈ (extract_Somes_gset s).
+  Proof. 
+    intros. rewrite /extract_Somes_gset.
+    rewrite elem_of_list_to_set. 
+    rewrite elem_of_list_In. rewrite -extract_Somes_spec.
+    rewrite -elem_of_list_In. rewrite elem_of_elements.
+    done. 
+  Qed.
+
+  Definition AM_live_roles {AM: ActionModel} `{Countable (amRole AM)} (AM_S: AM_strong_lr AM):
+    amSt AM -> gset (amRole AM) :=
+    extract_Somes_gset ∘ proj1_sig AM_S.
+
+  Lemma AM_live_roles_spec {AM: ActionModel} `{Countable (amRole AM)} (AM_S: AM_strong_lr AM):
+    forall st ρ,
+    (exists a st', amTrans st (a, Some ρ) st') <-> ρ ∈ AM_live_roles AM_S st.
+  Proof. 
+    intros. rewrite /AM_live_roles /compose.
+    rewrite -extract_Somes_gset_spec.
+    destruct AM_S as [f SPEC]. simpl. rewrite SPEC.
+    done.
+  Qed. 
+
+  Section AMProduct.
+    Context {AM1 AM2: ActionModel}.
+    Context {PA: Type}. 
+
+    (* TODO: should these types be isomorphic? *)
+    Context {fact_act: PA -> option (@amA AM1) * option (@amA AM2)}.
+
+    Let PS: Type := @amSt AM1 * @amSt AM2.
+    Let PR: Type := @amRole AM1 + @amRole AM2.
+
+    Inductive ProdTrans: PS -> PA * option PR -> PS -> Prop :=
+    | pt_inner1 s1 s1' s2 a1 r1 pa
+        (LBL: fact_act pa = (Some a1, None))
+        (STEP1: amTrans s1 (a1, Some r1) s1'):
+      ProdTrans (s1, s2) (pa, Some (inl r1)) (s1', s2)
+    | pt_inner2 s2 s2' s1 a2 r2 pa
+        (LBL: fact_act pa = (None, Some a2))
+        (STEP2: amTrans s2 (a2, Some r2) s2'):
+      ProdTrans (s1, s2) (pa, Some (inr r2)) (s1, s2')
+    | pt_sync1 s1 s1' s2 s2' a1 a2 r1 pa
+        (LBL: fact_act pa = (Some a1, Some a2))
+        (STEP1: amTrans s1 (a1, Some r1) s1')
+        (STEP2: amTrans s2 (a2, None) s2'):
+      ProdTrans (s1, s2) (pa, Some (inl r1)) (s1', s2')
+    | pt_sync2 s1 s1' s2 s2' a1 a2 r2 pa
+        (LBL: fact_act pa = (Some a1, Some a2))
+        (STEP1: amTrans s1 (a1, None) s1')
+        (STEP2: amTrans s2 (a2, Some r2) s2'):
+      ProdTrans (s1, s2) (pa, Some (inr r2)) (s1', s2')
+    .
+    
+    Definition ProdAM: ActionModel := {| amTrans := ProdTrans; |}.
+
+    (* Lemma ProdAM_strong_lr `{Countable (amRole AM1), Countable (amRole AM2)} *)
+    (*   {S1: AM_strong_lr AM1} {S2: AM_strong_lr AM1}:  *)
+    (*   AM_strong_lr ProdAM. *)
+    (* Proof.  *)
+    (*   destruct S1 as [lr1 S1], S2 as [lr2 S2].  *)
+
+    Lemma prod_AM_step_dec {EQ1: EqDecision (amSt AM1)} {EQ2: EqDecision (amSt AM2)}
+      (D1: AM_step_dec AM1) (D2: AM_step_dec AM2):      
+      AM_step_dec ProdAM.
+    Proof.
+      red. intros [s1 s2] a oρ [s1' s2'].
+      Ltac inv_step := right; intros S; inversion S; subst; congruence.
+      destruct oρ as [ρ| ]; [| inv_step]. 
+      destruct (fact_act a) as [oa1 oa2] eqn:F.
+      destruct oa1 as [a1| ], oa2 as [a2| ]; revgoals. 
+      { inv_step. }
+      - destruct ρ as [ρ1 | ρ2]. 
+        { inv_step. }
+        destruct (decide (s1' = s1)) as [-> | ?]; [| inv_step]. 
+        destruct (D2 s2 a2 (Some ρ2) s2'); [| inv_step]. 
+        left. econstructor; eauto.
+      - destruct ρ as [ρ1 | ρ2]. 
+        2: { inv_step. }
+        destruct (decide (s2' = s2)) as [-> | ?]; [| inv_step]. 
+        destruct (D1 s1 a1 (Some ρ1) s1'); [| inv_step]. 
+        left. econstructor; eauto.
+      - destruct ρ as [ρ1 | ρ2].
+        + destruct (D1 s1 a1 (Some ρ1) s1'), (D2 s2 a2 None s2').
+          2-4: inv_step.
+          left. econstructor; eauto.
+        + destruct (D1 s1 a1 None s1'), (D2 s2 a2 (Some ρ2) s2').
+          2-4: inv_step.
+          left. econstructor; eauto.
+    Qed.
+
+    (* TODO: move *)
+    Lemma ex_proper3 {A B C: Prop} (P Q: A -> B -> C -> Prop)
+      (EQUIV: forall a b c, P a b c <-> Q a b c):
+      (exists a b c, P a b c) <-> (exists a b c, Q a b c).
+    Proof.
+      set_solver.
+    Qed. 
+      
+    (* TODO: move *)
+    Lemma ex_prod' {A B: Type} (P: A -> B -> Prop):
+      (exists a b, P a b) <-> (exists ab, P ab.1 ab.2).
+    Proof.
+      split.
+      - intros (?&?&?). eexists (_, _). eauto.
+      - intros [[??] ?]. eauto.
+    Qed.
+
+    Lemma prod_AM_fin_branch' (FIN1: AM_fin_branch' AM1) (FIN2: AM_fin_branch' AM2)
+      inv_fact (INV: Cancel eq inv_fact fact_act)
+      :
+      AM_fin_branch' ProdAM.
+    Proof. 
+      destruct FIN1 as [ns1 FIN1], FIN2 as [ns2 FIN2].      
+      exists (fun '(s1, s2) =>
+           let l1 := (fun '(x, y, z) => (x, Some y, z)) <$> ns1 s1 in
+           let l2 := (fun '(x, y, z) => (x, Some y, z)) <$> ns2 s2 in 
+           '(s1', a1, oρ1) ← (s1, None, None) :: l1;
+           '(s2', a2, oρ2) ← (s2, None, None) :: l2;
+           let a' := inv_fact (a1, a2) in
+           ρ' ← [from_option (Some ∘ inl) None oρ1; from_option (Some ∘ inr) None oρ2];
+           mret ((s1', s2'), a', ρ')).
+      
+      intros [s1 s2] [s1' s2'] a oρ STEP.
+      pose proof (cancel_surj a) as [[oa1 oa2] EQ].
+      rewrite elem_of_list_bind.
+      rewrite !ex_prod.
+
+      (* TODO: shorten the following proof, rewrite under binders? *)
+      (* setoid_rewrite elem_of_list_bind. *)      
+
+      (* do 3 (eapply exist_proper; intros). *)
+      (* { pattern x1. match goal with |- ((fun y => ?F y <-> _) x1) => idtac "foo" end.  *)      
+
+      inversion STEP; subst.
+      { exists s1', (Some a1), (Some r1).
+        split.
+        2: { apply elem_of_cons. right. rewrite elem_of_list_fmap.
+             eexists. split; eauto. simpl. reflexivity. }
+        rewrite elem_of_list_bind.
+        exists (s2', None, None). 
+        rewrite elem_of_list_bind. split.
+        2: { apply elem_of_cons. tauto. }
+        exists (Some (inl r1)). simpl.
+        rewrite elem_of_list_ret. split; [| set_solver].
+        do 2 f_equal.
+        apply (@f_equal _ _ inv_fact) in LBL. by rewrite INV in LBL. }
+      { exists s1', None, None.
+        split.
+        2: { apply elem_of_cons. tauto. }
+        rewrite elem_of_list_bind.        
+        exists (s2', (Some a2), (Some r2)).
+        rewrite elem_of_list_bind. split.
+        2: { apply elem_of_cons. right. rewrite elem_of_list_fmap.
+             eexists. split; eauto. simpl. reflexivity. }
+        exists (Some (inr r2)). simpl.
+        rewrite elem_of_list_ret. split; [| set_solver].
+        do 2 f_equal.
+        apply (@f_equal _ _ inv_fact) in LBL. by rewrite INV in LBL. }  
+      { exists s1', (Some a1), (Some r1).
+        split.
+        2: { apply elem_of_cons. right. rewrite elem_of_list_fmap.
+             eexists. split; eauto. simpl. reflexivity. }
+        rewrite elem_of_list_bind.
+        exists (s2', Some a2, None). 
+        rewrite elem_of_list_bind. split.
+        2: { apply elem_of_cons. right. rewrite elem_of_list_fmap.
+             eexists. split; eauto. simpl. reflexivity. }
+        exists (Some (inl r1)). simpl.
+        rewrite elem_of_list_ret. split; [| set_solver].
+        do 2 f_equal.
+        apply (@f_equal _ _ inv_fact) in LBL. by rewrite INV in LBL. }
+      { exists s1', (Some a1), None.
+        split.
+        2: { apply elem_of_cons. right. rewrite elem_of_list_fmap.
+             eexists. split; eauto. simpl. reflexivity. }
+        rewrite elem_of_list_bind.
+        exists (s2', Some a2, Some r2). 
+        rewrite elem_of_list_bind. split.
+        2: { apply elem_of_cons. right. rewrite elem_of_list_fmap.
+             eexists. split; eauto. simpl. reflexivity. }
+        exists (Some (inr r2)). simpl.
+        rewrite elem_of_list_ret. split; [| set_solver].
+        do 2 f_equal.
+        apply (@f_equal _ _ inv_fact) in LBL. by rewrite INV in LBL. }
+    Qed. 
+
+  End AMProduct.
+
+  Section AM2FM.
+    Context (AM: ActionModel).
+    Context `{CNT_R: Countable (amRole AM)}. 
+    Context {EQ_ST: EqDecision (amSt AM)}. 
+    Context {INH_ST: Inhabited (amSt AM)} {INH_R: Inhabited (amRole AM)}.
+
+    (* this requirement is not necessary, but allows to reuse the AM_strong_lr machinery *)
+    Context (AM_S: AM_strong_lr AM). 
+
+    (* Context (am_lr: amSt AM -> gset (amRole AM)).  *)
+    (* Hypothesis (AM_LIVE_ROLES: forall s1 a ρ s2, amTrans s1 (a, Some ρ) s2 → ρ ∈ am_lr s1). *)
+
+    Inductive am_fmtrans: amSt AM → option (amRole AM) → amSt AM → Prop :=
+    | amfm_role_step s1 s2 a r (STEP: amTrans s1 (a, Some r) s2):
+      am_fmtrans s1 (Some r) s2
+    | amfm_env_step s1 s2 a (STEP: amTrans s1 (a, None) s2):
+      am_fmtrans s1 None s2
+    .
+
+    Definition AM2FM : FairModel.
+      refine {| fmtrans := am_fmtrans; live_roles := AM_live_roles AM_S |}.
+    Proof. 
+      intros. apply AM_live_roles_spec.
+      inversion H; eauto.
+    Defined. 
+
+  End AM2FM.  
+
+End ActionModel.
